Introduce `VariableState` in the interpreter and fix remainnig sorries (#599)
The idea is that getting/setting variables in a `VariableState` that is
contained in the `InterpreterState` makes things easier for proofs. This
is because we do not have to write many small lemmas about separation
between memory and variable states. In general, it just makes things
easier to manipulate.

Veir/Interpreter/Basic.lean
@@ -55,68 +55,71 @@ structure MemoryState where
 def MemoryState.empty : MemoryState :=
   { contents := (ByteArray.emptyWithCapacity 1024).extend 8 0xff }
 
+structure VariableState where
+  variables : Std.ExtHashMap ValuePtr RuntimeValue
+
 /--
   The state of the interpreter at a given point in time.
   It includes a mapping from IR values to their runtime values.
 -/
+@[ext]
 structure InterpreterState where
-  variables : Std.ExtHashMap ValuePtr RuntimeValue
+  variables : VariableState
   memory : MemoryState
 
 /--
   Set the value of a variable.
 -/
-def InterpreterState.setVar (state : InterpreterState) (var : ValuePtr) (val : RuntimeValue) :
-    InterpreterState :=
-  {state with variables := state.variables.insert var val}
+def VariableState.setVar (state : VariableState) (var : ValuePtr) (val : RuntimeValue) :
+    VariableState :=
+  ⟨state.variables.insert var val⟩
 
 /--
   Get the value of a variable, if the variable exists.
 -/
-def InterpreterState.getVar? (state : InterpreterState) (var : ValuePtr)
+def VariableState.getVar? (state : VariableState) (var : ValuePtr)
     : Option RuntimeValue :=
   state.variables[var]?
 
 @[ext]
-theorem InterpreterState.ext {s₁ s₂ : InterpreterState} :
+theorem VariableState.ext {s₁ s₂ : VariableState} :
     (∀ var, s₁.getVar? var = s₂.getVar? var) →
-    s₁.memory = s₂.memory →
     s₁ = s₂ := by
   rcases s₁; rcases s₂
-  simp only [getVar?, mk.injEq]
+  simp only [VariableState.getVar?, mk.injEq]
   grind
 
 /--
   Get the value of the operands of an operation.
   If any operand is not in the state, return `none`.
 -/
-def InterpreterState.getOperandValues (state : InterpreterState)
+def VariableState.getOperandValues (state : VariableState)
     (ctx : IRContext OpInfo) (op : OperationPtr) : Option (Array RuntimeValue) := do
   (op.getOperands! ctx).mapM state.getVar?
 
-def InterpreterState.setResultValues_loop (state : InterpreterState)
-    (ctx : IRContext OpInfo) (op : OperationPtr) (resultValues : Array RuntimeValue) (i : Nat) : InterpreterState :=
+def VariableState.setResultValues_loop (state : VariableState)
+    (ctx : IRContext OpInfo) (op : OperationPtr) (resultValues : Array RuntimeValue) (i : Nat) : VariableState :=
   match i with
   | 0 => state
   | i + 1 =>
     let result := op.getResult i
     let value := resultValues[i]!
     let newState := state.setVar result value
-    InterpreterState.setResultValues_loop newState ctx op resultValues i
+    VariableState.setResultValues_loop newState ctx op resultValues i
 
 /--
   Set the values of the results of an operation.
 -/
-def InterpreterState.setResultValues (state : InterpreterState) (ctx : IRContext OpInfo)
-    (op : OperationPtr) (resultValues : Array RuntimeValue) : InterpreterState :=
-  InterpreterState.setResultValues_loop state ctx op resultValues (op.getNumResults! ctx)
+def VariableState.setResultValues (state : VariableState) (ctx : IRContext OpInfo)
+    (op : OperationPtr) (resultValues : Array RuntimeValue) : VariableState :=
+  VariableState.setResultValues_loop state ctx op resultValues (op.getNumResults! ctx)
 
 /--
   Set the values of block arguments.
 -/
-def InterpreterState.setArgumentValues (state : InterpreterState) (ctx : IRContext OpInfo)
-    (block : BlockPtr) (values : Array RuntimeValue) : InterpreterState :=
-  let rec loop (state : InterpreterState) (i : Nat) :=
+def VariableState.setArgumentValues (state : VariableState) (ctx : IRContext OpInfo)
+    (block : BlockPtr) (values : Array RuntimeValue) : VariableState :=
+  let rec loop (state : VariableState) (i : Nat) :=
     match i with
     | 0 => state
     | i + 1 =>
@@ -130,7 +133,7 @@ def InterpreterState.setArgumentValues (state : InterpreterState) (ctx : IRConte
   Create an interpreter state with no variables defined.
 -/
 def InterpreterState.empty : InterpreterState :=
-  { variables := Std.ExtHashMap.emptyWithCapacity 8, memory := .empty }
+  { variables := ⟨Std.ExtHashMap.emptyWithCapacity 8⟩, memory := .empty }
 
 /--
   How the control flow should proceed after interpreting a terminator.
@@ -959,10 +962,10 @@ def interpretOp' (opType : OpCode) (properties : HasOpInfo.propertiesOf opType)
 -/
 def interpretOp (ctx : IRContext OpCode) (op : OperationPtr) (state : InterpreterState)
     : Interp (InterpreterState × Option ControlFlowAction) := do
-  let some operands := state.getOperandValues ctx op | none
+  let some operands := state.variables.getOperandValues ctx op | none
   let opType := op.getOpType! ctx
   let (resultValues, mem, action) ← interpretOp' opType (op.getProperties! ctx opType) (op.getResultTypes! ctx) operands (op.getSuccessors! ctx) state.memory
-  let newState := {state.setResultValues ctx op resultValues with memory := mem}
+  let newState := ⟨state.variables.setResultValues ctx op resultValues, mem⟩
   return (newState, action)
 
 /--
@@ -1005,7 +1008,7 @@ def interpretBlockCFG (ctx : IRContext OpCode) (blockPtr : BlockPtr) (state : In
   | some (.ok (state, .return res)) => some (.ok (state, res))
   | some (.ok (state, .branch res succ)) =>
     if h : succ.InBounds ctx then
-      let state := state.setArgumentValues ctx succ res
+      let state := ⟨state.variables.setArgumentValues ctx succ res, state.memory⟩
       interpretBlockCFG ctx succ state h wf else none
   | some .ub => Interp.ub
   | none => none
